src/Example.Compile.Pump.fst
@@ -1,5 +1,5 @@
 (* Compiling a simple example to C.
-   The program to translate is defined in Example.Check.Simple. *)
+   The program to translate is defined in Example.Check.Pump. *)
 module Example.Compile.Pump
 
 module Pump = Example.Check.Pump
@@ -16,7 +16,7 @@ open FStar.HyperStack.ST
    We do not want the expression's internal representation to show up in the
    C code, so we mark it as noextract. *)
 noextract
-let expr = (Pump.pump (Exp.XVar 0) (Exp.XVar 1) false)
+let expr = (Pump.controller (Exp.XVar 0) (Exp.XVar 1) false)
 
 (* Define the state type so it shows up as a type definition in the C code.
    The "postprocess_with" annotation ensures that the state_of_exp is inlined into the type and simplified to a regular type *)
@@ -24,12 +24,12 @@ let expr = (Pump.pump (Exp.XVar 0) (Exp.XVar 1) false)
 let state = XX.state_of_exp expr
 
 type input = {
-  estop_ok:  bool;
+  estop:     bool;
   level_low: bool;
 }
 
 type output = {
-  pump_en:   bool;
+  sol_en:   bool;
   nok_stuck: bool;
 }
 
@@ -44,6 +44,11 @@ let system: Pipit.Exec.Base.exec (int * (int * unit)) state int =
 [@@(Tac.postprocess_with XL.tac_extract)]
 let reset = XL.mk_reset system
 
+noextract
+let has_bit (i: int) (b: nat { b > 0 }) =
+  let open FStar.Mul in
+  (i % (b * 2)) >= b
+
 (* Define the step function, which takes two input integers and a pointer to the
    internal state, and returns the result as a bitfield. We parse the bitfield
    before returning the values.
@@ -52,6 +57,6 @@ let reset = XL.mk_reset system
 let step (inp: input) (stref: B.pointer state): ST output
     (requires (fun h -> B.live h stref))
     (ensures (fun h _ h' -> B.live h' stref)) =
-  let res = XL.mk_step system (Exp.value_of_bool inp.estop_ok, (Exp.value_of_bool inp.level_low, ())) stref in
+  let res = XL.mk_step system (Exp.value_of_bool inp.estop, (Exp.value_of_bool inp.level_low, ())) stref in
   // How to check bits on `int` type?
-  { pump_en = (res % 2) >= 1; nok_stuck = (res % 4) >= 2 }
+  { sol_en = has_bit res Pump.solenoid_flag; nok_stuck = has_bit res Pump.stuck_flag }
